proving grid soundness

GCSL.v
@@ -22,15 +22,30 @@ Definition default_stack : stack := fun x => 0%Z.
 Require Import MyVector.
 Import VectorNotations.
 
-Definition bdiv_g (gs : g_state nblk ntrd) :=
-  exists (bid : Fin.t nblk), 
-    Bdiv.bdiv ((blks gs)[@bid], sh_gl_heap (sh_hp gs)[@bid] (gl_hp gs)).
+Notation zpheap := (PHeap.gen_pheap Z).
+Notation zpheap' := (PHeap.gen_pheap' Z).
 
-Definition as_gheap (h : simple_heap) : heap :=
+Definition glist nblk ntrd := Vector.t (klist ntrd) nblk.
+
+Definition as_npgheap (h : simple_heap) : heap :=
   fun x => match x with
     | SLoc x => None
     | GLoc x => h x
   end.
+
+Definition as_gheap' (h : zpheap') : pheap' :=
+  fun x => match x with
+    | SLoc x => None
+    | GLoc x => h x
+  end.
+
+Lemma as_gh_is_ph (h : zpheap) : is_pheap (as_gheap' h).
+Proof.
+  intros [v | v]; unfold as_gheap'; eauto.
+  destruct h as [? isph]; simpl; specialize (isph v); auto.
+Qed.
+
+Definition as_gheap (h : zpheap) := Pheap (as_gh_is_ph h).
 
 Definition as_sheap (h : simple_heap) : heap :=
   fun x => match x with
@@ -38,22 +53,53 @@ Definition as_sheap (h : simple_heap) : heap :=
     | GLoc x => None
   end.    
 
-Fixpoint safe_ng (n : nat) (gs : g_state nblk ntrd) (Q : assn) :=
+Definition is_sheap (h : heap) := forall x, h (GLoc x) = None.
+Definition is_gheap (h : pheap') := forall x, h (SLoc x) = None.
+Lemma as_sh_is_sh (h : simple_heap) : is_sheap (as_sheap h).
+Proof.
+  unfold is_sheap; simpl; auto.
+Qed.
+Lemma as_gh_is_gh (h : zpheap) : is_gheap (as_gheap h).
+Proof.
+  unfold is_gheap; simpl; auto.
+Qed.
+
+Lemma sh_gh_disj (sh : heap) (gh : pheap') : is_sheap sh -> is_gheap gh -> pdisj (htop sh) gh.
+Proof.
+  unfold is_sheap, is_gheap, htop, htop'; intros; intros [? | ?]; simpl; auto;
+  try rewrite H; try rewrite H0; auto.
+  destruct (sh (SLoc z)); auto.
+Qed.
+Hint Resolve sh_gh_disj as_sh_is_sh as_gh_is_gh.
+Lemma sh_gl_is_ph (sh : simple_heap) (gh : zpheap) : pdisj (htop (as_sheap sh)) (as_gheap gh).
+Proof.
+  auto.
+Qed.
+
+Definition sh_gl_pheap (sh : simple_heap) (gh : zpheap) : pheap := phplus_pheap (sh_gl_is_ph sh gh).
+
+Definition bdiv_g (gs : glist nblk ntrd) (shs : Vector.t simple_heap nblk) (gh : zpheap) :=
+  exists (bid : Fin.t nblk), 
+    Bdiv.bdiv (gs[@bid], (sh_gl_pheap shs[@bid] gh)).
+
+Fixpoint safe_ng (n : nat) (gs : glist nblk ntrd)
+         (shs : Vector.t simple_heap nblk) (gh : zpheap) (Q : assn) :=
   match n with
     | 0 => True
     | S n =>
-      ((forall (bid : Fin.t nblk) (tid : Fin.t ntrd), fst ((blks gs)[@bid][@tid]) = SKIP) ->
-         Q default_stack (htop (as_gheap (gl_hp gs)))) /\
-      (forall hF : simple_heap,
-         hdisj (gl_hp gs) hF ->
-         ~abort_g (Gs (blks gs) (sh_hp gs) (hplus (gl_hp gs) hF))) /\
-      ~ bdiv_g gs /\ 
-      (forall (gs' : g_state nblk ntrd) (hF : simple_heap),
-         hdisj (gl_hp gs) hF ->
-         red_g (Gs (blks gs) (sh_hp gs) (hplus (gl_hp gs) hF)) gs' ->
-         exists (h'' : simple_heap),
-           hdisj h'' hF /\ (gl_hp gs') = hplus h'' hF /\
-           safe_ng n (Gs (blks gs') (sh_hp gs') h'') Q)
+      ((forall (bid : Fin.t nblk) (tid : Fin.t ntrd), fst gs[@bid][@tid] = SKIP) ->
+         Q default_stack (as_gheap gh)) /\
+      (forall (hF : zpheap) (h : simple_heap),
+         pdisj gh hF ->
+         ptoheap (phplus gh hF) h -> ~abort_g (Gs gs shs h)) /\
+      ~ bdiv_g gs shs gh /\ 
+      (forall (gs' : g_state nblk ntrd) (hF : zpheap) (h : simple_heap),
+         pdisj gh hF ->
+         ptoheap (phplus gh hF) h ->
+         red_g (Gs gs shs h) gs' ->
+         exists (h'' : zpheap),
+           pdisj h'' hF /\ ptoheap (phplus h'' hF) (gl_hp gs') /\
+           safe_ng n (blks gs') (sh_hp gs') h'' Q)
   end.
 
 Record program : Set := Pr {
@@ -93,23 +139,22 @@ Section For_List_Notation.
   Definition has_no_vars (P : assn) : Prop := indeP (fun (_ _ : stack) => True) P.
   
   Lemma safe_gl (n : nat) :
-    forall (gs : g_state nblk ntrd) (ghs : Vector.t heap nblk) (Q : assn) (sh_decl : list (var * nat) )
+    forall (gs : glist nblk ntrd) (shs : Vector.t simple_heap nblk) (gh : zpheap) (ghs : Vector.t zpheap nblk) (Q : assn) (sh_decl : list (var * nat) )
            (Qs : Vector.t assn nblk),
       let sinv := sh_spec sh_decl in
-      disj_eq (Vector.map (@htop loc) ghs) (htop (as_gheap (gl_hp gs))) ->
+      disj_eq ghs gh ->
       (forall bid : Fin.t nblk,
-         safe_nk E n (fst (bs_of_gs gs bid))
-                 (hplus (as_sheap (sh_hp gs)[@bid]) ghs[@bid]) (sinv ** Qs[@bid])) ->
+         safe_nk E n gs[@bid] (sh_gl_pheap shs[@bid] ghs[@bid]) (sinv ** Qs[@bid])) ->
       (forall bid : Fin.t nblk, has_no_vars Qs[@bid]) ->
       Aistar_v Qs |= Q -> 
-      (forall bid tid, sinv (snd (blks gs)[@bid][@tid]) (htop (as_sheap (sh_hp gs)[@bid]))) ->
-      (forall bid tid, inde sinv (writes_var (fst (blks gs)[@bid][@tid]))) ->
+      (forall bid tid, sinv (snd gs[@bid][@tid]) (htop (as_sheap shs[@bid]))) ->
+      (forall bid tid, inde sinv (writes_var (fst gs[@bid][@tid]))) ->
       (forall var, List.In var (List.map fst sh_decl) -> E var = Lo) ->
-      safe_ng n gs Q.
+      safe_ng n gs shs gh Q.
   Proof.
     induction n; [simpl; auto|].
     remember (safe_nk E (S n)).
-    simpl; intros gs ghs Q sdec Qs Hdeq Hsafe Hnov HQ Hsinv Hsvar Hslow; repeat split; subst.
+    simpl; intros gs shs gh ghs Q sdec Qs Hdeq Hsafe Hnov HQ Hsinv Hsvar Hslow; repeat split; subst.
     - intros Hskip.
       evar (P : Fin.t nblk -> Prop); assert (Hskipb : forall bid, P bid); [|unfold P in *; clear P].
       { unfold P; intros bid; destruct (Hsafe bid) as (Hskipb & _).
@@ -133,27 +178,12 @@ Section For_List_Notation.
             unfold low_eq in Hlow; unfold_conn_all; simpl in *; intros x; rewrite <-Hlow; auto.
         Qed.
 
-        assert ((sh_spec sdec) srep (htop (as_sheap (sh_hp gs)[@bid]))).
+        assert ((sh_spec sdec) srep (htop (as_sheap shs[@bid]))).
         { assert (exists nt, ntrd = S nt) as [nt Hnt] by (exists (ntrd - 1); omega).
           generalize dependent gs; rewrite Hnt; intros.
-          apply (sh_spec_inde _ (snd (blks gs)[@bid][@Fin.F1]) _ E); auto.
+          apply (sh_spec_inde _ (snd gs[@bid][@Fin.F1]) _ E); auto.
           specialize (Hsrep Fin.F1); erewrite nth_map in Hsrep; [apply Hsrep|]; auto. }
 
-        Definition is_sheap (h : heap) := forall x, h (GLoc x) = None.
-        Definition is_gheap (h : heap) := forall x, h (SLoc x) = None.
-        Lemma as_sh_is_sh (h : simple_heap) : is_sheap (as_sheap h).
-        Proof.
-          unfold is_sheap; simpl; auto.
-        Qed.
-        Lemma as_gh_is_gh (h : simple_heap) : is_gheap (as_gheap h).
-        Proof.
-          unfold is_gheap; simpl; auto.
-        Qed.
-
-        Lemma sh_gh_disj (sh gh : heap) : is_sheap sh -> is_gheap gh -> hdisj sh gh.
-        Proof.
-          unfold is_sheap, is_gheap; intros; intros [? | ?]; auto.
-        Qed.
 
         Lemma htop_hplus (h1 h2 : heap) (H : hdisj h1 h2) :
           (htop (hplus h1 h2)) = phplus_pheap (proj1 (hdisj_pdisj h1 h2) H).
@@ -166,55 +196,53 @@ Section For_List_Notation.
 
         Require Import Program.
         
-        Lemma disj_eq_inj n (hs : Vector.t heap n) :forall h,
-          disj_eq (Vector.map (@htop _) hs) (htop h) ->
-          is_gheap h -> forall i, is_gheap hs[@i].
-        Proof.
-          induction n; simpl; intros h H Hgh i.
-          - inversion i.
-          - dependent destruction hs; dependent destruction i; simpl in *.
-            + intros l.
-              inversion H; subst; simpl; auto.
-              apply (f_equal (fun x => x (SLoc l))) in H4; unfold phplus, htop' in H4.
-              specialize (Hgh l).
-              destruct ph as [ph ?]; simpl in *.
-              destruct (h (SLoc l)), (ph (SLoc l)) as [[? ?]|], (h0 (SLoc l)); congruence.
-            + remember (htop h0) as hh0; inversion H; subst; simpl in *.
-              apply Eqdep.EqdepTheory.inj_pair2 in H3; subst; eauto.
-              apply (f_equal (fun x => this x)) in H2; simpl in H2.
+        (* Lemma disj_eq_inj n (hs : Vector.t heap n) :forall h, *)
+        (*   disj_eq (Vector.map (@htop _) hs) (htop h) -> *)
+        (*   is_gheap h -> forall i, is_gheap hs[@i]. *)
+        (* Proof. *)
+        (*   induction n; simpl; intros h H Hgh i. *)
+        (*   - inversion i. *)
+        (*   - dependent destruction hs; dependent destruction i; simpl in *. *)
+        (*     + intros l. *)
+        (*       inversion H; subst; simpl; auto. *)
+        (*       apply (f_equal (fun x => x (SLoc l))) in H4; unfold phplus, htop' in H4. *)
+        (*       specialize (Hgh l). *)
+        (*       destruct ph as [ph ?]; simpl in *. *)
+        (*       destruct (h (SLoc l)), (ph (SLoc l)) as [[? ?]|], (h0 (SLoc l)); congruence. *)
+        (*     + remember (htop h0) as hh0; inversion H; subst; simpl in *. *)
+        (*       apply Eqdep.EqdepTheory.inj_pair2 in H3; subst; eauto. *)
+        (*       apply (f_equal (fun x => this x)) in H2; simpl in H2. *)
 
-              Lemma htop_phplus_heap (h1 h2 : heap) (ph : pheap) :
-                pdisj (htop h1) ph ->
-                phplus (htop' h1) ph = htop' h2 ->
-                exists ph', ph = htop ph'.
-              Proof.
-                intros;exists (fun x => match PHeap.this ph x with None => None | Some (_,x) => Some x end).
-                destruct ph as [ph ?]; apply pheap_eq.
-                unfold phplus, htop, htop' in *; simpl in *; extensionality x;
-                apply (f_equal (fun f => f x)) in H0.
-                specialize (is_p x); specialize (H x).
-                pose proof frac_contra1.
-                destruct (ph x) as [[? ?]|], (h1 x), (h2 x); first [now auto | congruence | firstorder].
-              Qed.
+        (*       Lemma htop_phplus_heap (h1 h2 : heap) (ph : pheap) : *)
+        (*         pdisj (htop h1) ph -> *)
+        (*         phplus (htop' h1) ph = htop' h2 -> *)
+        (*         exists ph', ph = htop ph'. *)
+        (*       Proof. *)
+        (*         intros;exists (fun x => match PHeap.this ph x with None => None | Some (_,x) => Some x end). *)
+        (*         destruct ph as [ph ?]; apply pheap_eq. *)
+        (*         unfold phplus, htop, htop' in *; simpl in *; extensionality x; *)
+        (*         apply (f_equal (fun f => f x)) in H0. *)
+        (*         specialize (is_p x); specialize (H x). *)
+        (*         pose proof frac_contra1. *)
+        (*         destruct (ph x) as [[? ?]|], (h1 x), (h2 x); first [now auto | congruence | firstorder]. *)
+        (*       Qed. *)
 
-              pose proof (@htop_phplus_heap _ _ _ hdis H2) as [ht Hht]; subst; auto.
-              eapply IHn.
-              apply H4.
+        (*       pose proof (@htop_phplus_heap _ _ _ hdis H2) as [ht Hht]; subst; auto. *)
+        (*       eapply IHn. *)
+        (*       apply H4. *)
 
-              intros x; apply (f_equal (fun f => f (SLoc x))) in H2; specialize (Hgh x).
-              unfold phplus, htop, htop' in H2; simpl in H2.
-              repeat lazymatch type of H2 with
-                | context [match ?X with | Some _ => _ | None => _ end] => destruct X
-                | context [let (_, _) := ?X in _] => destruct X
-              end; try congruence.
-        Qed.
+        (*       intros x; apply (f_equal (fun f => f (SLoc x))) in H2; specialize (Hgh x). *)
+        (*       unfold phplus, htop, htop' in H2; simpl in H2. *)
+        (*       repeat lazymatch type of H2 with *)
+        (*         | context [match ?X with | Some _ => _ | None => _ end] => destruct X *)
+        (*         | context [let (_, _) := ?X in _] => destruct X *)
+        (*       end; try congruence. *)
+        (* Qed. *)
 
-        assert (hdisj (as_sheap (sh_hp gs)[@bid]) ghs[@bid]).
-        { apply sh_gh_disj; [apply as_sh_is_sh|].
-          apply disj_eq_inj with (as_gheap (gl_hp gs)); auto.
-          apply as_gh_is_gh. }
+
+        assert (pdisj (htop (as_sheap shs[@bid])) (as_gheap ghs[@bid])) by auto.
         
-        rewrite htop_hplus with (H :=H1) in H.
+        (* rewrite htop_hplus with (H :=H1) in H. *)
 
         Lemma sc_cancel (P Q : assn) s (hp hq : pheap) (Hdis : pdisj hp hq) :
           precise P ->
@@ -315,104 +343,175 @@ Section For_List_Notation.
           apply Eqdep.EqdepTheory.inj_pair2 in H4; subst; auto.
       Qed.
 
+      Lemma as_gheap_pdisj (h1 h2 : zpheap) :
+        pdisj h1 h2 -> pdisj (as_gheap h1) (as_gheap h2).
+      Proof.
+        intros H; intros [l | l]; simpl; auto.
+        specialize (H l); auto.
+      Qed.
+      Hint Resolve as_gheap_pdisj.
+      
+      Lemma phplus_as_gheap (h1 h2 : zpheap') :
+        pdisj h1 h2 ->
+        as_gheap' (phplus h1 h2) = phplus (as_gheap' h1) (as_gheap' h2).
+      Proof.
+        intros H.
+        extensionality x; destruct x; unfold hplus; simpl; auto.
+      Qed.        
+
+      Lemma disj_eq_as_gh {n : nat} (hs : Vector.t zpheap n) (h : zpheap) :
+        disj_eq hs h -> disj_eq (Vector.map as_gheap hs) (as_gheap h).
+      Proof.
+        dependent induction hs; intros Heq; inversion Heq; subst.
+        - assert (as_gheap (emp_ph Z) = emp_ph loc).
+          { apply pheap_eq; extensionality l; destruct l as [l | l]; unfold emp_h; eauto. }
+          rewrite H; constructor.
+        - apply Eqdep.EqdepTheory.inj_pair2 in H2; subst.
+          assert (Hdis : pdisj (as_gheap h) (as_gheap ph)) by auto.
+          assert (as_gheap (Pheap (pdisj_is_pheap hdis)) = phplus_pheap Hdis).
+          { lets Heq': (>>phplus_as_gheap hdis); unfold phplus_pheap in Heq'.
+            apply pheap_eq; simpl; auto. }
+          rewrite H; constructor; eauto.
+      Qed.          
+      apply disj_eq_as_gh in Hdeq.
       eapply aistar_sat; eauto.
       intros; erewrite Vector.nth_map; [|reflexivity]; auto.
 
-    - intros hF Hdis [bid ?].
+    - intros hF h Hdis Heq [bid ?].
       destruct (Hsafe bid) as (_ & Hnabort & _ & _).
       unfold bs_of_gs in H; simpl in H.
       
       Lemma sh_gl_heap_hplus (h1 h2 : simple_heap) :
-        sh_gl_heap h1 h2 = hplus (as_sheap h1) (as_gheap h2).
+        sh_gl_heap h1 h2 = hplus (as_sheap h1) (as_npgheap h2).
       Proof.
         extensionality l; destruct l; unfold hplus; simpl; auto.
         destruct (h1 z); auto.
       Qed.
 
-      rewrite sh_gl_heap_hplus in H.
-      
-      Lemma hplus_assoc {loc : Type} (h1 h2 h3 : PHeap.heap loc) :
-        hplus (hplus h1 h2) h3 = hplus h1 (hplus h2 h3).
+      Lemma phplus_is_gheap (h1 h2 : pheap') :
+        is_gheap h1 -> is_gheap h2 -> is_gheap (phplus h1 h2).
       Proof.
-        extensionality l; unfold hplus.
-        destruct (h1 l); auto.
-      Qed.
-
-      Lemma hplus_as_gheap (h1 h2 : simple_heap) :
-        as_gheap (hplus h1 h2) = hplus (as_gheap h1) (as_gheap h2).
-      Proof.
-        extensionality x; destruct x; unfold hplus; simpl; auto.
-      Qed.        
-
-      rewrite hplus_as_gheap, <-hplus_assoc in H.
-      Lemma is_sheap_disj h1 h2 h3 :
-        is_sheap h1 -> is_gheap h2 -> is_gheap h3 ->
-        hdisj h2 h3 -> hdisj (hplus h1 h2) h3.
-      Proof.
-        intros; intros l.
-        destruct l; specialize (H z); specialize (H0 z); specialize (H1 z).
-        unfold hplus; auto.
-        unfold hplus; rewrite H; auto.
-      Qed.
-
-      Lemma as_gheap_hdisj (h1 h2 : simple_heap) :
-        hdisj h1 h2 -> hdisj (as_gheap h1) (as_gheap h2).
-      Proof.
-        intros; intros [l | l]; simpl; auto.
-      Qed.
-      
-      Lemma hdisjC {loc : Type} (h1 h2 : PHeap.heap loc) : hdisj h1 h2 -> hdisj h2 h1.
-      Proof.
-        intros; intros l; specialize (H l); tauto.
-      Qed.
-      
-      assert (Hgb_gh : is_gheap ghs[@bid]).
-      { eapply disj_eq_inj; eauto using as_gh_is_gh. }
-      
-      apply disjeq_phplus with (i := bid) (h' := htop (as_gheap hF)) in Hdeq.
-      2: apply hdisj_pdisj.
-      2: apply as_gheap_hdisj; auto.
-      destruct Hdeq as (hF' & Hdis1 & Hdis2 & Heq1 & Hdisj3).
-      erewrite Vector.nth_map in Heq1; [|reflexivity].
-      assert (exists hhF', hF' = htop hhF') as [hhF' HF']; subst.
-      { eapply htop_phplus_heap.
-        erewrite Vector.nth_map in Hdis1; [|reflexivity..].
-        apply Hdis1.
-        apply Heq1. }
-      rewrite <-hplus_phplus in Heq1; simpl in Heq1; auto.
-      rewrite <-heap_pheap_eq in Heq1.
-      rewrite <-Heq1 in H. 
-      Infix "|+|" := hplus (at level 40, left associativity).
-      assert (as_sheap (sh_hp gs)[@bid] |+| (ghs[@bid] |+| hhF') |+| as_gheap hF =
-              hplus (hplus (as_sheap (sh_hp gs)[@bid]) ghs[@bid]) (hplus hhF' (as_gheap hF))).
-      { rewrite !hplus_assoc; auto. }
-      rewrite H0 in H; apply Hnabort in H; auto.
-      erewrite Vector.nth_map in Hdisj3; [|reflexivity].
-      rewrite <-hplus_phplus in Hdisj3.
-
-      Lemma hplus_is_gheapC (h1 h2 h : heap) :
-        is_gheap h2 -> h1 |+| h = h2 -> is_gheap h.
-      Proof.
-        unfold is_gheap; intros.
-        apply (f_equal (fun f => f (SLoc x))) in H0; unfold hplus in H0; simpl.
-        specialize (H x).
-        destruct (h1 (SLoc x)), (h2 (SLoc x)); try rewrite H in *; try congruence.
-      Qed.
-      
-      Lemma hplus_is_gheap (h1 h2 : heap) :
-        is_gheap h1 -> is_gheap h2 -> is_gheap (h1 |+| h2).
-      Proof.
-        unfold is_gheap, hplus; intros; rewrite H, H0; auto.
+        unfold is_gheap, phplus; intros; rewrite H, H0; auto.
       Qed.
         
-      apply is_sheap_disj; auto using as_sh_is_sh, as_gh_is_gh.
-      apply hplus_is_gheap; auto using as_sh_is_sh, as_gh_is_gh.
-      apply hplus_is_gheapC in Heq1; auto using as_gh_is_gh.
-      apply hdisj_pdisj; auto.
-      apply hdisj_pdisj; auto.
-      apply hdisj_pdisj; auto.
-      erewrite Vector.nth_map in Hdis1; [|reflexivity].
-      auto.
+      Hint Resolve pdisjE1 pdisjE2 sh_gh_disj phplus_is_gheap.
+      lets (hrest & _ & Hdis0 & Heq0): (>> disj_tid bid Hdeq).
+      assert (HdisrF : pdisj hrest hF).
+      { rewrite <-Heq0 in Hdis; apply pdisjC, pdisjE2, pdisjC in Hdis; auto. }
+      assert (pdisj (sh_gl_pheap shs[@bid] ghs[@bid]) (as_gheap (phplus_pheap HdisrF))).
+      { apply pdisj_padd_expand; auto; split.
+        apply sh_gh_disj; auto.
+        apply as_gheap_pdisj, pdisj_padd_expand; auto.
+        rewrite Heq0; auto. }
+      lets Hna: (>> Hnabort (sh_gl_heap shs[@bid] h) H0); applys Hna; auto.
+      
+      Lemma eq_ptoheap (h : heap) (ph : pheap') :
+        ph = htop h -> ptoheap ph h.
+      Proof.
+        intros H l; rewrite H; unfold htop, htop'; simpl.
+        destruct (h l); eauto.
+      Qed.
+      apply eq_ptoheap.
+
+      Lemma htop_sh_gl_heap (h1 h2 : simple_heap) :
+        htop (sh_gl_heap h1 h2) = sh_gl_pheap h1 (htop h2).
+      Proof.
+        apply pheap_eq; unfold sh_gl_heap, as_sheap, as_gheap, phplus, htop, htop'.
+        extensionality l; destruct l as [l|l]; simpl.
+        destruct (h1 l); eauto.
+        destruct (h2 l); eauto.
+      Qed.
+      assert (pdisj ghs[@bid] (phplus hrest hF)).
+      { apply pdisj_padd_expand; eauto.
+        rewrite Heq0; auto. }
+      rewrite sh_gl_heap_hplus in H; eauto.
+      rewrite htop_sh_gl_heap; unfold sh_gl_pheap; eauto.
+      Notation this := PHeap.this.
+      cutrewrite (this (phplus_pheap (sh_gl_is_ph shs[@bid] ghs[@bid])) =
+                  phplus (htop (as_sheap shs[@bid])) (as_gheap ghs[@bid])); auto.
+      rewrite padd_assoc; eauto.
+      cutrewrite (this (phplus_pheap (sh_gl_is_ph shs[@bid] (htop h))) =
+                  phplus (htop (as_sheap shs[@bid])) (as_gheap (htop h))); auto.
+      f_equal.
+      simpl; rewrite <-phplus_as_gheap; eauto.
+      f_equal.
+      rewrite <-padd_assoc; eauto.
+      cutrewrite (phplus gh hF = phplus_pheap Hdis) in Heq; auto.
+      rewrite Heq0.
+      apply ptoheap_eq in Heq; apply (f_equal (fun x => this x)) in Heq; auto.
+      
+      (* Lemma hplus_assoc {loc : Type} (h1 h2 h3 : PHeap.heap loc) : *)
+      (*   hplus (hplus h1 h2) h3 = hplus h1 (hplus h2 h3). *)
+      (* Proof. *)
+      (*   extensionality l; unfold hplus. *)
+      (*   destruct (h1 l); auto. *)
+      (* Qed. *)
+
+      (* Lemma hplus_as_gheap (h1 h2 : simple_heap) : *)
+      (*   hdisj h1 h2 -> *)
+      (*   as_npgheap (hplus h1 h2) = hplus (as_npgheap h1) (as_gheap h2). *)
+      (* Proof. *)
+      (*   apply pheap_eq. *)
+      (*   extensionality x; destruct x; unfold hplus; simpl; auto. *)
+      (* Qed.         *)
+
+      (* rewrite hplus_as_gheap, <-hplus_assoc in H. *)
+      (* Lemma is_sheap_disj h1 h2 h3 : *)
+      (*   is_sheap h1 -> is_gheap h2 -> is_gheap h3 -> *)
+      (*   hdisj h2 h3 -> hdisj (hplus h1 h2) h3. *)
+      (* Proof. *)
+      (*   intros; intros l. *)
+      (*   destruct l; specialize (H z); specialize (H0 z); specialize (H1 z). *)
+      (*   unfold hplus; auto. *)
+      (*   unfold hplus; rewrite H; auto. *)
+      (* Qed. *)
+      
+      (* Lemma hdisjC {loc : Type} (h1 h2 : PHeap.heap loc) : hdisj h1 h2 -> hdisj h2 h1. *)
+      (* Proof. *)
+      (*   intros; intros l; specialize (H l); tauto. *)
+      (* Qed. *)
+      
+      (* assert (Hgb_gh : is_gheap ghs[@bid]). *)
+      (* { eapply disj_eq_inj; eauto using as_gh_is_gh. } *)
+      
+      (* apply disjeq_phplus with (i := bid) (h' := htop (as_gheap hF)) in Hdeq. *)
+      (* 2: apply hdisj_pdisj. *)
+      (* 2: apply as_gheap_hdisj; auto. *)
+      (* destruct Hdeq as (hF' & Hdis1 & Hdis2 & Heq1 & Hdisj3). *)
+      (* erewrite Vector.nth_map in Heq1; [|reflexivity]. *)
+      (* assert (exists hhF', hF' = htop hhF') as [hhF' HF']; subst. *)
+      (* { eapply htop_phplus_heap. *)
+      (*   erewrite Vector.nth_map in Hdis1; [|reflexivity..]. *)
+      (*   apply Hdis1. *)
+      (*   apply Heq1. } *)
+      (* rewrite <-hplus_phplus in Heq1; simpl in Heq1; auto. *)
+      (* rewrite <-heap_pheap_eq in Heq1. *)
+      (* rewrite <-Heq1 in H.  *)
+      Infix "|+|" := hplus (at level 40, left associativity).
+      (* assert (as_sheap (sh_hp gs)[@bid] |+| (ghs[@bid] |+| hhF') |+| as_gheap hF = *)
+      (*         hplus (hplus (as_sheap (sh_hp gs)[@bid]) ghs[@bid]) (hplus hhF' (as_gheap hF))). *)
+      (* { rewrite !hplus_assoc; auto. } *)
+      (* rewrite H0 in H; apply Hnabort in H; auto. *)
+      (* erewrite Vector.nth_map in Hdisj3; [|reflexivity]. *)
+      (* rewrite <-hplus_phplus in Hdisj3. *)
+
+      (* Lemma hplus_is_gheapC (h1 h2 h : heap) : *)
+      (*   is_gheap h2 -> h1 |+| h = h2 -> is_gheap h. *)
+      (* Proof. *)
+      (*   unfold is_gheap; intros. *)
+      (*   apply (f_equal (fun f => f (SLoc x))) in H0; unfold hplus in H0; simpl. *)
+      (*   specialize (H x). *)
+      (*   destruct (h1 (SLoc x)), (h2 (SLoc x)); try rewrite H in *; try congruence. *)
+      (* Qed. *)
+      
+      (* apply is_sheap_disj; auto using as_sh_is_sh, as_gh_is_gh. *)
+      (* apply hplus_is_gheap; auto using as_sh_is_sh, as_gh_is_gh. *)
+      (* apply hplus_is_gheapC in Heq1; auto using as_gh_is_gh. *)
+      (* apply hdisj_pdisj; auto. *)
+      (* apply hdisj_pdisj; auto. *)
+      (* apply hdisj_pdisj; auto. *)
+      (* erewrite Vector.nth_map in Hdis1; [|reflexivity]. *)
+      (* auto. *)
       
     - intros Hbdiv; destruct Hbdiv as [bid Hbdiv].
       destruct (Hsafe bid) as (_ & _ & Hbdivi & _).
@@ -426,29 +525,80 @@ Section For_List_Notation.
       Proof.
         unfold hdisj; intros; destruct (h x); auto.
       Qed.
-      specialize (Hbdivi emp_h); rewrite emp_h_unit_r in Hbdivi; auto; apply Hbdivi in Hbdiv;
-      auto using emp_h_disj.
+      eapply bdiv_weaken in Hbdiv; eauto.
+      (* specialize (Hbdivi emp_h); rewrite emp_h_unit_r in Hbdivi; auto; apply Hbdivi in Hbdiv; *)
+      (* auto using emp_h_disj. *)
 
-    - intros gs' hF Hdis Hred.
+    - intros gs' hF h Hdis Heq Hred.
       inversion Hred; subst; simpl; clear Hred.
       rename H into Hred; rename H0 into Hheq.
       unfold bs_of_gs in Hred; simpl in Hred.
       rewrite sh_gl_heap_hplus in Hred.
-      assert (exists hb, as_gheap (gl_hp gs) = hplus ghs[@bid] hb /\
-                         hdisj ghs[@bid] hb) as (hb & Hhb & Hdishb).
-      { apply (disj_tid bid) in Hdeq as (hb & ? & ? & ?).
-        erewrite Vector.nth_map in H1, H0; [|reflexivity..].
-        assert (exists hb', hb = htop hb') as (hb' & ?); subst.
-        { simpl in H1; apply htop_phplus_heap in H1; auto. }
-        rewrite <-hdisj_pdisj in H0.
-        rewrite <-hplus_phplus in H1; simpl in H1; auto.
-        rewrite <-heap_pheap_eq in H1.
-        exists hb'; split; auto. }
-      assert (Heq : as_sheap (sh_hp gs)[@bid] |+| as_gheap (gl_hp gs |+| hF) =
-                    (as_sheap (sh_hp gs)[@bid] |+| ghs[@bid]) |+| (hb |+| as_gheap hF)).
-      { rewrite hplus_as_gheap, Hhb, !hplus_assoc; auto. }
-      rewrite Heq in Hred; clear Heq.
+      lets (hb & _ & Hdisr & Heqr): (>>disj_tid bid Hdeq).
+      (* assert (exists hb, gh = phplus ghs[@bid] hb /\ *)
+      (*                    pdisj ghs[@bid] hb) as (hb & Hhb & Hdishb). *)
+      (* { apply (disj_tid bid) in Hdeq as (hb & ? & ? & ?). *)
+      (*   erewrite Vector.nth_map in H1, H0; [|reflexivity..]. *)
+      (*   assert (exists hb', hb = htop hb') as (hb' & ?); subst. *)
+      (*   { simpl in H1; apply htop_phplus_heap in H1; auto. } *)
+      (*   rewrite <-hdisj_pdisj in H0. *)
+      (*   rewrite <-hplus_phplus in H1; simpl in H1; auto. *)
+      (*   rewrite <-heap_pheap_eq in H1. *)
+      (*   exists hb'; split; auto. } *)
       destruct (Hsafe bid) as (_ & _ & _ & _ & Hsafei).
+      assert (HdisbF : pdisj hb hF).
+      { rewrite <-Heqr in Hdis; apply pdisjC, pdisjE2, pdisjC in Hdis; eauto. }
+      lets (ph'' & Hdis'' & Heq'' & Hsafe''): (>> Hsafei (phplus_pheap (as_gheap_pdisj _ _ HdisbF)) Hred).
+      { apply pdisj_padd_expand; eauto; split; eauto.
+        apply sh_gh_disj; eauto.
+        apply phplus_is_gheap; eauto.
+        apply phplus_is_gheap; eauto.
+        apply pdisj_padd_expand; eauto.
+        simpl; rewrite <-phplus_as_gheap, Heqr; eauto.
+        apply as_gheap_pdisj; eauto. }
+      { apply eq_ptoheap.
+        unfold sh_gl_pheap.
+        cutrewrite (this (phplus_pheap (sh_gl_is_ph shs[@bid] ghs[@bid])) =
+                    phplus (htop (as_sheap shs[@bid])) (as_gheap ghs[@bid])); auto.
+        rewrite padd_assoc; eauto.
+        Lemma htop_as_npgheap h:
+          htop' (as_npgheap h) = as_gheap (htop h).
+        Proof.
+          extensionality l; destruct l as [l | l]; unfold htop', as_npgheap, as_gheap';
+          eauto.
+        Qed.
+        assert (hdisj (as_sheap shs[@bid]) (as_npgheap h)).
+        { apply hdisj_pdisj; simpl.
+          rewrite htop_as_npgheap.
+          apply sh_gl_is_ph. }
+        rewrite (htop_hplus _ _ H); eauto.
+        simpl; f_equal.
+        cutrewrite (phplus gh hF = phplus_pheap Hdis) in Heq; auto.
+        apply ptoheap_eq in Heq; apply (f_equal (fun x => this x)) in Heq; simpl in Heq.
+        rewrite <-Heqr in Heq.
+        rewrite htop_as_npgheap; eauto.
+        rewrite <-!phplus_as_gheap; simpl; f_equal; eauto.
+        rewrite <-padd_assoc; eauto.
+
+        (* 残り *)
+        apply pdisj_padd_expand; eauto.
+        rewrite Heqr; eauto.
+        apply pdisj_padd_expand; eauto.
+        rewrite Heqr; eauto.
+        apply sh_gh_disj; eauto.
+        repeat apply phplus_is_gheap; eauto.
+        simpl.
+        rewrite <-phplus_as_gheap; eauto.
+        cutrewrite (phplus hb hF = phplus_pheap HdisbF); auto.
+        apply as_gheap_pdisj.
+        apply pdisj_padd_expand; eauto.
+        rewrite Heqr; eauto. }
+      
+        assert (Heq : as_sheap shs[@bid] |+| as_npgheap h =
+                      (as_sheap (sh_hp gs)[@bid] |+| ghs[@bid]) |+| (hb |+| as_gheap hF)).
+        { rewrite hplus_as_gheap, Hhb, !hplus_assoc; auto. }
+        rewrite Heq in Hred; clear Heq.
+
       
       assert (hdisj (as_sheap (sh_hp gs)[@bid] |+| ghs[@bid]) (hb |+| as_gheap hF)).
       { apply is_sheap_disj; auto using as_sh_is_sh, as_gh_is_gh.
@@ -618,7 +768,7 @@ Section For_List_Notation.
 
       + intros; rewrite !replace_nth; destruct fin_eq_dec; eauto. 
 
-        Notation this := PHeap.this.
+
         Definition dom_eqp (h1 h2 : pheap) :=
           forall (l : loc) p,
             (exists v, this h1 l = Some (p, v)) <->
